Defined through EdgeSetPathEq, using the RPath definition from util.v
Took the definition of RPath (and the two variations, RPath', RPath'')
and moved forward, using this to define EdgePaths and EdgeEqPaths.

Changed some naming conventions slightly. PredEdges are now
StrandEdges. They're the edges that make a strand. This seemed more
direct to their meaning. Also, before I had a somewhat confusing way of
labeling the relations that also included membership in a specific set
(I had tried, for example, CommEdge' and CommEdge_). These are now
[EdgeType]SetEdge (e.g. CommSetEdge), thus making them very explicit
and self explanatory. I also changed SSEdge (Strand Space Edge) to
XEdge (as in "x" the variable, as in *either* a comm or strand edge).
StrandSpaceEdge seems like the most accurate, but is painfully lengthy
(can you imagine StrandSpaceSetEdgeEq?). SSEdge is what I was using,
which when combined with SetEdges make SSSetEdge… which is painful. I
guess I could do GraphEdge, GEdge, CSEdge (Comm [or] Strand Edge?), or
stick with SSEdge and just deal with SSSetEdge… All of these feel
varyingly gross… which is driving me nuts. Oh well, 'XEdge' it is for
this push.

strands2.v
@@ -183,13 +183,13 @@ Proof.
   intros X l i. generalize dependent l.
   induction i. 
   Case "length <= 0".
-  intros l H.
-  unfold nth_error in H. unfold error in H.
-  destruct l. auto. inversion H.
+    intros l H.
+    unfold nth_error in H. unfold error in H.
+    destruct l. auto. inversion H.
   Case "length <= S i".
-  intros l' H.
-  destruct l'. simpl; omega.
-  inversion H. apply IHi in H1. simpl. omega. 
+    intros l' H.
+    destruct l'. simpl; omega.
+    inversion H. apply IHi in H1. simpl. omega. 
 Qed.
 
 Theorem node_smsg_valid : 
@@ -236,7 +236,7 @@ Proof.
 Qed.
 
 Inductive CommEdge : relation Node :=
-| cedge :  forall x y t, ((Node_smsg x = tx t /\
+| comm_edge :  forall x y t, ((Node_smsg x = tx t /\
                            Node_smsg y = rx t)
                         /\ Node_strand x <> Node_strand y)
                         -> CommEdge x y.
@@ -253,24 +253,32 @@ Hint Constructors CommEdge.
   its own transmission by any reasonable measure. *)
 
 (* A CommEdge between nodes, where the set the nodes belong to is specified. *)
-Inductive CommEdge_ : Nodes -> relation Node :=
-| cedge_ : forall N x y,
+Inductive CommSetEdge : Nodes -> relation Node :=
+| comm_sedge : forall N x y,
               In x N ->
               In y N ->
               CommEdge x y ->
-              CommEdge_ N x y.
-Hint Constructors CommEdge_.
+              CommSetEdge N x y.
+Hint Constructors CommSetEdge.
 
-Theorem cedge_imp_neq : forall n m,
+Theorem comm_edge_imp_neq : forall n m,
  CommEdge n m -> n <> m.
  Proof.
    intros n m Hedge Hneq. subst.
    inversion Hedge as [contra_s contra_i]; subst.
    apply H. reflexivity.
  Qed.  
-Hint Resolve cedge_imp_neq.
+Hint Resolve comm_edge_imp_neq.
 
-Theorem cedge_antisymmetry : 
+Theorem comm_edge_refl_false : forall m,
+ CommEdge m m -> False.
+Proof.
+  intros m edge.
+  apply comm_edge_imp_neq in edge.
+  apply edge. reflexivity.
+Qed.
+
+Theorem comm_edge_antisymmetry : 
 antisymmetric Node CommEdge.
 Proof.
   intros n m Hcomm contra.
@@ -280,80 +288,98 @@ Proof.
   destruct H0 as [H Hneq_s2]. destruct H as [Htx2 Hrx2].
   rewrite Htx2 in Hrx1. inversion Hrx1.
 Qed.
-Hint Resolve cedge_antisymmetry.
+Hint Resolve comm_edge_antisymmetry.
 
-(* predecessor edge *)
-(* node's direct predecessor -> node -> Prop *)
-Inductive PredEdge : relation Node :=
-| pedge : forall i j, Node_strand i = Node_strand j 
+(* strand edge *)
+(* Edge representing a node, and the node proceeding it on the same strand. *)
+Inductive StrandEdge : relation Node :=
+| strand_edge : forall i j, Node_strand i = Node_strand j 
                        -> (Node_index i) + 1 = Node_index j 
-                       -> PredEdge i j.
+                       -> StrandEdge i j.
 (* [REF 1] Definition 2.3.4 pg 6
    "When n1= <s,i> and n2=<s,i+1> are members of N (set of node), there is
     an edge n1 => n2." *)
 
-(* An CommEdge between nodes, where the set the nodes belong to is specified. *)
-Inductive PredEdge_ : Nodes -> relation Node :=
-| pedge_ : forall N x y,
+(* An Strand Edge between nodes, where the set the nodes belong to is specified. *)
+Inductive StrandSetEdge : Nodes -> relation Node :=
+| strand_sedge : forall N x y,
               In x N ->
               In y N ->
-              PredEdge x y ->
-              PredEdge_ N x y.
-Hint Constructors PredEdge_.
+              StrandEdge x y ->
+              StrandSetEdge N x y.
+Hint Constructors StrandSetEdge.
 
-Theorem pedge_imp_neq : forall (n m: Node),
-PredEdge n m -> n <> m.
+Theorem strand_edge_imp_neq : forall (n m: Node),
+StrandEdge n m -> n <> m.
 Proof.
   intros n m Hedge Heq.
   subst. inversion Hedge; subst.
   omega.
 Qed.
-Hint Resolve pedge_imp_neq.
+Hint Resolve strand_edge_imp_neq.
 
-Theorem pedge_antisymmetry :
-antisymmetric Node PredEdge.
+Theorem strand_edge_refl_false : forall m,
+StrandEdge m m -> False.
+Proof.
+  intros m edge.
+  apply strand_edge_imp_neq in edge.
+  apply edge. reflexivity.
+Qed.
+
+Theorem strand_edge_antisymmetry :
+antisymmetric Node StrandEdge.
 Proof.
   intros n m Hpe1 Hpe2.
   destruct Hpe1. destruct Hpe2.
   rewrite <- H0 in H2. omega.
 Qed.
-Hint Resolve pedge_antisymmetry.
+Hint Resolve strand_edge_antisymmetry.
 
-Definition PredPath (l:list Node) : TPath PredEdge l.
+(* A Path representing the transitive closure of StrandEdge. *)
+Definition StrandPath (l:list Node) : RPath StrandEdge l.
 
-(*
-TODO?
+(* A Path representing the transitive closure of PredEdge, starting from x. *)
+Definition StrandPath' (l: list Node) (x: Node) : RPath' StrandEdge l x.
 
-PredPath' x ->* ...
-PredPath'' x ->* y
+(* A Path representing a path of PredEdges from x to y. *)
+Definition StrandPath'' (l: list Node) (x y: Node) : RPath'' StrandEdge l x y.
 
-*)
+Definition XEdge : relation Node := 
+union Node CommEdge StrandEdge.
 
-Definition SSEdge : relation Node := 
-union Node CommEdge PredEdge.
-
-Inductive SSEdge_ : Nodes -> relation Node :=
-| ssedge_ : forall N x y,
+Inductive XSetEdge : Nodes -> relation Node :=
+| x_sedge : forall N x y,
                In x N ->
                In y N ->
-               SSEdge x y ->
-               SSEdge_ N x y.
+               XEdge x y ->
+               XSetEdge N x y.
 
-Theorem ssedge_imp_neq : forall (n m:Node),
-SSEdge n m -> n <> m.
+Inductive XEdgeEq : relation Node :=
+| x_edge_eq_refl : forall x, XEdgeEq x x
+| x_edge_eq_step : forall x y, XEdge x y -> XEdgeEq x y.
+
+Inductive XSetEdgeEq : Nodes -> relation Node :=
+| x_sedge_eq : forall N x y,
+               In x N ->
+               In y N ->
+               XEdgeEq x y ->
+               XSetEdgeEq N x y.
+
+Theorem x_edge_imp_neq : forall (n m:Node),
+XEdge n m -> n <> m.
 Proof.
   intros n m Hedge Heq.
   inversion Hedge; subst.
-  apply (cedge_imp_neq m m); auto.
-  apply (pedge_imp_neq m m); auto.
+  apply (comm_edge_imp_neq m m); auto.
+  apply (strand_edge_imp_neq m m); auto.
 Qed.
 
-Theorem ssedge_antisymmetry :
-antisymmetric Node SSEdge.
+Theorem x_edge_antisymmetry :
+antisymmetric Node XEdge.
 Proof.
   intros n m Hss Hcontra.
   inversion Hss; subst. inversion Hcontra; subst.
-  apply (cedge_antisymmetry n m H) in H0. exact H0.
+  apply (comm_edge_antisymmetry n m H) in H0. exact H0.
   assert False.
   inversion H; subst. inversion H0; subst.
   inversion H1. apply H5. symmetry. exact H2.
@@ -362,9 +388,46 @@ Proof.
   inversion Hcontra; subst. inversion H; subst.
   inversion H0; subst. inversion H3. apply H5.
   symmetry. exact H1.
-  remember (pedge_antisymmetry n m H). apply e in H0.  
-  remember (pedge_imp_neq n m H). 
+  remember (strand_edge_antisymmetry n m H). apply e in H0.  
+  remember (strand_edge_imp_neq n m H). 
   contradiction. inversion H0.
 Qed.
 
-Definition EdgePath (l:list Node) : TPath SSEdge l.
+Definition EdgePath (l:list Node) : RPath XEdge l.
+
+Definition EdgeSetPath (l:list Node) (N: Nodes) : RPath (XSetEdge N) l.
+
+Definition EdgePathEq (l:list Node) : RPath XEdgeEq l.
+
+Definition EdgeSetPathEq (l:list Node) (N: Nodes) : RPath (XSetEdgeEq N) l.
+
+(* Next - Acyclic EdgePath
+  previously this was 
+
+Inductive Acyclic_Node : Node -> Prop :=
+| acyc_node : forall n,  ~(EdgePath n n) -> Acyclic_Node n.
+
+Inductive Acyclic_Nodes : Nodes -> Prop :=
+| acyclic_nodes : forall N,  
+                    (forall n, In Node N n -> 
+                                Acyclic_Node n) -> Acyclic_Nodes N.
+
+Two questions to answer before proceeding:
+  1) Does it Need to be specified as a prop? Can we just have a theorem
+     that is provable from just the definition of EdgePath? It seems like
+     if an EdgePath had a cycle, you would get a contradiction based on 
+     strand indices at a min
+  2) How should this be specified? Specifically for this case? More
+     Generally for RPaths?
+
+ALSO
+ - The RPath definition seems to be okay/working. Is it ideal? Is there some
+   obvious problem? Or improvement?
+
+Also ALSO - I would like to prove an equivalence between the natural transitive
+ and reflexive-transitive closures we were using originally, and these RPath
+ versions if possible. It would be, it feels, very useful to be able to show
+ one implies the other and be able to hop back and forth depending on what I'm
+ trying to prove (Could be wrong... but this seems reasonable...)
+
+*)
